imp/definition/ImpPrelude.v
@@ -8,6 +8,7 @@ Require Export ITreelib.
 Require Export AList.
 Require Import Skeleton.
 Require Import ModSem.
+Require Orders List.
 
 Set Implicit Arguments.
 
@@ -43,6 +44,219 @@ Global Program Instance EMSConfigImp: EMSConfig := {|
   initial_arg := ([]: list val)↑;
 |}
 .
+
+Module ImpSkel.
+  Import Orders List.
+
+  Inductive gdef: Type := Gfun | Gvar (gv: Z).
+
+  Module GDef <: Typ. Definition t := gdef. End GDef.
+  Module SkSort := AListSort GDef.
+
+  Definition sort: alist gname gdef -> alist gname gdef := SkSort.sort.
+
+  Program Definition gdefs: Sk.ld :=
+    @Sk.mk (alist gname gdef) nil (@List.app _) sort (fun sk => @List.NoDup _ (List.map fst sk)) _ _ _ _ _ _ _.
+  Next Obligation.
+  Proof.
+    eapply SkSort.sort_add_comm. auto.
+    (* eapply Permutation.Permutation_NoDup; [|et]. *)
+    (* eapply Permutation.Permutation_map. *)
+    (* symmetry. eapply SkSort.sort_permutation. *)
+  Qed.
+  Next Obligation.
+  Proof.
+    eapply List.app_assoc.
+  Qed.
+  Next Obligation.
+  Proof.
+    rewrite List.app_nil_r. auto.
+  Qed.
+  Next Obligation.
+  Proof.
+    i. eapply Permutation.Permutation_NoDup; [|et].
+    eapply Permutation.Permutation_map.
+    apply Permutation.Permutation_app_comm.
+  Qed.
+  Next Obligation.
+  Proof.
+    econs.
+  Qed.
+  Next Obligation.
+  Proof.
+    cut (NoDup (map fst a)).
+    { i. eapply Permutation.Permutation_NoDup; [|et].
+      eapply Permutation.Permutation_map.
+      eapply SkSort.sort_permutation. }
+    cut (NoDup (map fst (a ++ b))).
+    { i. rewrite map_app in H0.
+      eapply nodup_app_l. et. }
+    i. eapply Permutation.Permutation_NoDup; [|et].
+    eapply Permutation.Permutation_map.
+    symmetry. eapply SkSort.sort_permutation.
+  Qed.
+
+Local Existing Instance gdefs.
+
+  Definition sort_add_comm sk0 sk1
+             (WF: Sk.wf (Sk.add sk0 sk1))
+    :
+      sort (Sk.add sk0 sk1) = sort (Sk.add sk1 sk0).
+  Proof.
+    eapply SkSort.sort_add_comm. eapply WF.
+  Qed.
+
+
+  Definition sort_wf sk (WF: Sk.wf sk):
+    Sk.wf (sort sk).
+  Proof.
+    ss. eapply Permutation.Permutation_NoDup; [|apply WF].
+    eapply Permutation.Permutation_map.
+    eapply SkSort.sort_permutation.
+  Qed.
+
+  (*** TODO: It might be nice if Sk.t also constitutes a resource algebra ***)
+  (*** At the moment, List.app is not assoc/commutative. We need to equip RA with custom equiv. ***)
+
+  Definition load_skenv (sk: Sk.t): SkEnv.t :=
+    let n := List.length sk in
+    {|
+      SkEnv.mblock := nat;
+      SkEnv.ptrofs := Z;
+      SkEnv.blk2id := fun blk => do '(gn, _) <- (List.nth_error sk blk); Some gn;
+      SkEnv.id2blk := fun id => do '(blk, _) <- find_idx (fun '(id', _) => string_dec id id') sk; Some blk
+    |}
+  .
+
+  Lemma load_skenv_wf sk
+        (WF: Sk.wf sk)
+    :
+      <<WF: SkEnv.wf (load_skenv sk)>>
+  .
+  Proof.
+    r in WF.
+    rr. split; i; ss.
+    - uo; des_ifs.
+      + f_equal. ginduction sk; ss. i. inv WF.
+        rewrite find_idx_red in Heq1. des_ifs; ss.
+        { des_sumbool. subst. ss. clarify. }
+        des_sumbool. uo. des_ifs. destruct p. ss.
+        hexploit IHsk; et.
+      + exfalso. ginduction sk; ss. i. inv WF.
+        rewrite find_idx_red in Heq2. des_ifs; ss.
+        des_sumbool. uo. des_ifs. destruct p. ss.
+        hexploit IHsk; et.
+    - ginduction sk; ss.
+      { i. uo. ss. destruct blk; ss. }
+      i. destruct a. inv WF. uo. destruct blk; ss; clarify.
+      {  rewrite find_idx_red. uo. des_ifs; des_sumbool; ss. }
+      hexploit IHsk; et. i.
+      rewrite find_idx_red. uo. des_ifs; des_sumbool; ss. exfalso.
+      subst. clear - Heq1 H2. ginduction sk; ss. i.
+      rewrite find_idx_red in Heq1. des_ifs; des_sumbool; ss; et.
+      uo. des_ifs. destruct p. eapply IHsk; et.
+  Qed.
+
+  Definition incl (sk0 sk1: Sk.t): Prop :=
+    forall gn gd (IN: List.In (gn, gd) sk0),
+      List.In (gn, gd) sk1.
+
+  Program Instance incl_PreOrder: PreOrder incl.
+  Next Obligation.
+  Proof.
+    ii. ss.
+  Qed.
+  Next Obligation.
+  Proof.
+    ii. eapply H0. eapply H. ss.
+  Qed.
+
+  Lemma sort_incl sk
+    :
+      incl sk (sort sk).
+  Proof.
+    ii. eapply Permutation.Permutation_in; [|apply IN].
+    eapply SkSort.sort_permutation.
+  Qed.
+
+  Lemma sort_incl_rev sk
+    :
+      incl (sort sk) sk.
+  Proof.
+    ii. eapply Permutation.Permutation_in; [|apply IN].
+    symmetry. eapply SkSort.sort_permutation.
+  Qed.
+
+  Definition incl_env (sk0: Sk.t) (skenv: SkEnv.t): Prop :=
+    forall gn gd (IN: List.In (gn, gd) sk0),
+    exists blk, <<FIND: skenv.(SkEnv.id2blk) gn = Some blk>>.
+
+  Lemma incl_incl_env sk0 sk1
+        (INCL: incl sk0 sk1)
+    :
+      incl_env sk0 (load_skenv sk1).
+  Proof.
+    ii. exploit INCL; et. i. ss. uo. des_ifs; et.
+    exfalso. clear - x0 Heq0. ginduction sk1; et.
+    i. ss. rewrite find_idx_red in Heq0. des_ifs.
+    des_sumbool. uo.  des_ifs. des; clarify.
+    eapply IHsk1; et.
+  Qed.
+
+  Lemma in_env_in_sk :
+    forall sk blk symb
+      (FIND: @SkEnv.blk2id (load_skenv sk) blk = Some symb),
+    exists def, In (symb, def) sk.
+  Proof.
+    i. unfold SkEnv.blk2id. ss.
+    uo. des_ifs. des; clarify.
+    eapply nth_error_In in Heq0. et.
+  Qed.
+
+  Lemma in_sk_in_env :
+    forall sk def symb
+           (IN: In (symb, def) sk),
+    exists blk, @SkEnv.blk2id (load_skenv sk) blk = Some symb.
+  Proof.
+    i. unfold SkEnv.blk2id. ss.
+    uo. eapply In_nth_error in IN. des.
+    eexists. rewrite IN. et.
+  Qed.
+
+  Lemma env_range_some :
+    forall sk blk
+      (BLKRANGE : blk < Datatypes.length sk),
+      <<FOUND : exists symb, @SkEnv.blk2id (load_skenv sk) blk = Some symb>>.
+  Proof.
+    i. depgen sk. induction blk; i; ss; clarify.
+    { destruct sk; ss; clarify.
+      { lia. }
+      uo. destruct p. exists s. ss. }
+    destruct sk; ss; clarify.
+    { lia. }
+    apply lt_S_n in BLKRANGE. eapply IHblk; eauto.
+  Qed.
+
+  Lemma env_found_range :
+    forall sk symb blk
+      (FOUND : @SkEnv.id2blk (load_skenv sk) symb = Some blk),
+      <<BLKRANGE : blk < Datatypes.length sk>>.
+  Proof.
+    induction sk; i; ss; clarify.
+    uo; des_ifs. destruct p0. rewrite find_idx_red in Heq0. des_ifs.
+    { apply Nat.lt_0_succ. }
+    destruct blk.
+    { apply Nat.lt_0_succ. }
+    uo. des_ifs. destruct p. ss. clarify. apply lt_n_S. eapply IHsk; eauto.
+    instantiate (1:=symb). rewrite Heq0. ss.
+  Qed.
+
+End ImpSkel.
+
+Import ImpSkel.
+
+Global Existing Instance gdefs.
+
 
 Definition wordsize_64 := 64.
 Definition modulus_64 := two_power_nat wordsize_64.
@@ -103,8 +317,6 @@ Definition vmul (x y: val): option val :=
   | _, _ => None
   end
 .
-
-
 
 
 
@@ -181,9 +393,9 @@ Module Mem.
       (fun blk ofs =>
          do '(g, gd) <- (List.nth_error sk blk);
          match gd with
-         | Sk.Gfun =>
+         | Gfun =>
            None
-         | Sk.Gvar gv =>
+         | Gvar gv =>
            if csl g then None else
            if (dec ofs 0%Z) then Some (Vint gv) else None
          end)
