spc/Hoareproof2.v
@@ -3,6 +3,8 @@ Require Import STS.
 Require Import Behavior.
 Require Import ModSem.
 Import ModSemL.
+Require Import ImpPrelude.
+Import ImpSkel.
 Require Import Skeleton.
 Require Import PCM.
 Require Import Any.
@@ -38,7 +40,7 @@ Section CANCEL.
 
   Variable mds: list SMod.t.
 
-  Let sk: Sk.t := Sk.sort (fold_right Sk.add Sk.unit (List.map SMod.sk mds)).
+  Let sk: Sk.t := ImpSkel.sort (fold_right Sk.add Sk.unit (List.map SMod.sk mds)).
   (* Let skenv: SkEnv.t := Sk.load_skenv sk. *)
   Let mss: list SModSem.t := (List.map ((flip SMod.get_modsem) sk) mds).
   Let sbtb: list (gname * fspecbody) := (List.flat_map (SModSem.fnsems) mss).
@@ -95,7 +97,7 @@ Section CANCEL.
     Beh.of_program (ModL.compile (Mod.add_list mds_src)).
   Proof.
     eapply ModSem.refines_close.
-    eapply (@adequacy_local_list_strong mds_src mds_mid2).
+    eapply (@adequacy_local_list_strong _ mds_src mds_mid2).
     unfold mds_src, mds_mid2.
     eapply Forall2_apply_Forall2.
     { refl. }
